lib/Lib.Endianness.fsti
@@ -2,7 +2,6 @@ module Lib.Endianness
 
 open FStar.HyperStack
 open FStar.HyperStack.ST
-
 open LowStar.Buffer
 
 open Lib.IntTypes
@@ -10,27 +9,29 @@ open Lib.RawIntTypes
 open Lib.Buffer
 
 module B = LowStar.Buffer
-module ByteSeq = Lib.ByteSequence
+module BS = Lib.ByteSequence
+
+
 
 inline_for_extraction
 val uint_from_bytes_le:
     #t:m_inttype{~(SIZE? t)}
   -> i:lbuffer uint8 (numbytes t)
   -> Stack (uint_t t)
-    (requires fun h0 -> B.live h0 i)
+    (requires fun h0 -> live h0 i)
     (ensures  fun h0 o h1 ->
-      h0 == h1 /\ B.live h1 i /\
-      o == ByteSeq.uint_from_bytes_le #t (B.as_seq h0 i))
+      h0 == h1 /\ live h1 i /\
+      o == BS.uint_from_bytes_le #t (as_seq h0 i))
 
 inline_for_extraction
 val uint_from_bytes_be:
     #t:m_inttype{~(SIZE? t)}
   -> i:lbuffer uint8 (numbytes t)
   -> Stack (uint_t t)
-    (requires fun h0 -> B.live h0 i)
+    (requires fun h0 -> live h0 i)
     (ensures  fun h0 o h1 ->
-      h0 == h1 /\ B.live h1 i /\
-      o == ByteSeq.uint_from_bytes_be #t (B.as_seq h0 i))
+      h0 == h1 /\ live h1 i /\
+      o == BS.uint_from_bytes_be #t (as_seq h0 i))
 
 inline_for_extraction
 val uint_to_bytes_le:
@@ -38,10 +39,10 @@ val uint_to_bytes_le:
   -> o:lbuffer uint8 (numbytes t)
   -> i:uint_t t
   -> Stack unit
-    (requires fun h0 -> B.live h0 o)
+    (requires fun h0 -> live h0 o)
     (ensures  fun h0 _ h1 ->
-      B.live h1 o /\ modifies (loc_buffer o) h0 h1 /\
-      B.as_seq h1 o == ByteSeq.uint_to_bytes_le #t i)
+      live h1 o /\ modifies (loc_buffer o) h0 h1 /\
+      as_seq h1 o == BS.uint_to_bytes_le #t i)
 
 inline_for_extraction
 val uint_to_bytes_be:
@@ -49,7 +50,64 @@ val uint_to_bytes_be:
   -> o:lbuffer uint8 (numbytes t)
   -> i:uint_t t
   -> Stack unit
-    (requires fun h0 -> B.live h0 o)
+    (requires fun h0 -> live h0 o)
     (ensures  fun h0 _ h1 ->
-      B.live h1 o /\ modifies (loc_buffer o) h0 h1 /\
-      B.as_seq h1 o == ByteSeq.uint_to_bytes_be #t i)
+      live h1 o /\ modifies (loc_buffer o) h0 h1 /\
+      as_seq h1 o == BS.uint_to_bytes_be #t i)
+
+inline_for_extraction
+val uints_from_bytes_le:
+  #t:m_inttype
+  -> #len:size_nat{len `op_Multiply` numbytes t <= max_size_t}
+  -> o:lbuffer (uint_t t) len
+  -> clen:size_t{size_v clen == len}
+  -> i:lbuffer uint8 (len `op_Multiply` (numbytes t)) ->
+  Stack unit
+	(requires (fun h0 -> live h0 o /\ live h0 i))
+	(ensures (fun h0 _ h1 -> modifies (loc_buffer o) h0 h1 /\
+			      as_seq h1 o ==
+			      (BS.uints_from_bytes_le #t #(len) (as_seq h0 i) )))
+
+inline_for_extraction
+val uints_from_bytes_be:
+  #t:m_inttype -> #len:size_nat{len `op_Multiply` numbytes t <= max_size_t} ->
+  o:lbuffer (uint_t t) len ->
+  clen:size_t{size_v clen == len} ->
+  i:lbuffer uint8 (len `op_Multiply` ((numbytes t))) ->
+  Stack unit
+	(requires (fun h0 -> live h0 o /\ live h0 i))
+	(ensures (fun h0 _ h1 -> modifies (loc_buffer o) h0 h1 /\
+			      as_seq h1 o ==
+			      (BS.uints_from_bytes_be #t #(len) (as_seq h0 i) )))
+
+inline_for_extraction
+val uints_to_bytes_le:
+  #t:m_inttype
+  -> #len:size_nat{len `op_Multiply` numbytes t <= max_size_t}
+  -> o:lbuffer uint8 (len `op_Multiply` ((numbytes t)))
+  -> clen:size_t{size_v clen == len}
+  -> i:lbuffer (uint_t t) len ->
+  Stack unit
+	(requires (fun h0 -> live h0 o /\ live h0 i))
+	(ensures (fun h0 _ h1 -> modifies (loc_buffer o) h0 h1 /\
+			      as_seq h1 o ==
+			      (BS.uints_to_bytes_le #t #len (as_seq h0 i) )))
+
+inline_for_extraction
+val uints_to_bytes_be:
+    #t:m_inttype
+  -> #len:size_nat{len `op_Multiply` numbytes t <= max_size_t}
+  -> o:lbuffer uint8 (len `op_Multiply` (numbytes t))
+  -> clen:size_t{size_v clen == len}
+  -> i:lbuffer (uint_t t) len ->
+  Stack unit
+	(requires (fun h0 -> live h0 o /\ live h0 i /\ disjoint o i))
+	(ensures (fun h0 _ h1 -> modifies (loc_buffer o) h0 h1 /\
+			      as_seq h1 o ==
+			      (BS.uints_to_bytes_be #t #len (as_seq h0 i) )))
+
+inline_for_extraction
+let uint32s_to_bytes_le = uints_to_bytes_le #U32
+
+inline_for_extraction
+let uint32s_from_bytes_le = uints_from_bytes_le #U32
